Significant progress on Lemma body_uint63_to_nat

examples/uint63nat/prims_verif.v
@@ -65,21 +65,16 @@ Proof.
       forward.
       { entailer!. }
       entailer!.  
-      Search Int64.shl.
       autorewrite with norm.
       f_equal. unfold encode_Z. 
-      Search Int64.shl Int64.one. unfold encode_Z in H. unfold Int64.max_signed in H. 
+      unfold encode_Z in H. unfold Int64.max_signed in H. 
       autorewrite with norm. 
-      Search Int64.shl. 
       rewrite Int64.shl_mul_two_p. autorewrite with norm. unfold two_p. 
       unfold two_power_pos. 
       rewrite !Int.signed_repr; try rep_lia. 
       f_equal. 
       split; try rep_lia. unfold max_signed in *. unfold Int.max_signed. clear - H. simpl in *.
-      Locate "*".
-      Search Z.mul.
       rewrite Z.mul_comm in H. 
-      Search Z.le Z.mul.
 
       (* Todo: Work on postcondition. *)
      admit.
@@ -96,8 +91,8 @@ Proof.
   forward_call (gv, g). 
    assert ( Vlong (Int64.shru (Int64.repr (encode_Z (Z.of_nat n))) (Int64.repr (Int.unsigned (Int.repr 1)))) = Vlong (Int64.repr  (Z.of_nat n)))  as ->.
     { unfold encode_Z. 
-    autorewrite with norm. Search Int64.shru . rewrite Int64.shru_div_two_p. 
-    unfold two_p.  Search Int64.unsigned Int64.repr. simpl. 
+    autorewrite with norm. rewrite Int64.shru_div_two_p. 
+    unfold two_p. simpl. 
     
     admit. (* TODO *)  } 
   (*   Print bool_type. *)
@@ -109,8 +104,9 @@ Proof.
   gc_graph_iso g roots g' roots)
    LOCAL (temp _temp (rep_type_val g' v);
    temp _i (Vlong (Int64.repr (Z.of_nat (n - m))));
-   temp _tinfo ti; temp _t (Vlong (Int64.repr (Z.of_nat n))))
-   SEP (full_gc g' t_info' roots outlier ti sh)
+   temp _tinfo ti; temp _t (Vlong (Int64.repr (Z.of_nat n)));
+   gvars gv)
+   SEP (full_gc g' t_info' roots outlier ti sh gv)
   ). 
 
   - (* Before the while *)
@@ -153,95 +149,462 @@ all: fail.
 Admitted.
 
 
+#[export] Instance CCE: change_composite_env env_graph_gc.CompSpecs CompSpecs.
+make_cs_preserve env_graph_gc.CompSpecs CompSpecs.
+Defined.
 
-Lemma body_uint63_to_nat_spec :
+Lemma full_gc_fold:
+  forall gv g t_info roots outlier ti sh,
+  gc_condition_prop g t_info roots outlier ->
+   spatial_gcgraph.outlier_rep outlier *
+   before_gc_thread_info_rep sh t_info ti *
+   spatial_gcgraph.ti_token_rep (ti_heap t_info) (ti_heap_p t_info) * 
+   spatial_gcgraph.graph_rep g *
+   gc_spec.all_string_constants Ers gv
+  |--   full_gc g (t_info: GCGraph.thread_info) roots outlier ti sh gv.
+Proof. intros. unfold full_gc. entailer!!.
+Qed.
+
+Definition frame_rep (fr vr prev: val) (al: list val) :=
+  (*  fr is the address of the frame struct; vr is the local array address;
+      prev is the previous top-of-stack; al is the list of valid values
+  *)
+  (data_at Tsh (Tstruct _stack_frame noattr)
+    (offset_val (sizeof(int_or_ptr_type)*Zlength al) vr, (vr, prev)) fr
+   * data_at Tsh (tarray int_or_ptr_type (Zlength al)) al vr)%logic.
+
+Definition frame_rep_ (fr vr prev: val) (n: Z) :=
+  (*  fr is the address of the frame struct; vr is the local array address;
+      prev is the previous top-of-stack; n is the size of the local array;
+      there are no valid values at present
+  *)
+  (data_at Tsh (Tstruct _stack_frame noattr)
+    (Vundef, (vr, prev)) fr
+   * data_at_ Tsh (tarray int_or_ptr_type n) vr)%logic.
+
+Definition frame_rep_surplus (fr vr: val) (n: Z) (al: list val) :=
+   !! field_compatible (tarray int_or_ptr_type n) [] vr 
+   && data_at_ Tsh (tarray int_or_ptr_type (n-Zlength al))
+       (field_address0 (tarray int_or_ptr_type n) [ArraySubsc (Zlength al)] vr) .
+
+Lemma frame_rep_fold: forall fr vr prev n al,
+  Zlength al <= n ->
+  data_at Tsh (Tstruct _stack_frame noattr)
+    (offset_val (sizeof(int_or_ptr_type)*Zlength al) vr, (vr, prev)) fr
+   * data_at Tsh (tarray int_or_ptr_type n) (al++Zrepeat Vundef (n-Zlength al)) vr
+  |-- frame_rep fr vr prev al
+      * frame_rep_surplus fr vr n al.
+Proof.
+intros. unfold frame_rep, frame_rep_surplus.
+ entailer!.
+ erewrite split2_data_at_Tarray_app.
+ 2: reflexivity. 2: list_solve.
+ cancel.
+Qed.
+
+Lemma frame_rep__fold: forall fr vr prev n any,
+    data_at Tsh (Tstruct _stack_frame noattr) (any, (vr, prev)) fr
+   * data_at_ Tsh (tarray int_or_ptr_type n) vr
+  |-- frame_rep_ fr vr prev n.
+Proof. intros. unfold frame_rep_. cancel.
+  do 2 unfold_data_at (data_at _ _ _ _). cancel.
+Qed.
+
+#[export] Instance CCE2: change_composite_env env_graph_gc.CompSpecs CompSpecs.
+make_cs_preserve env_graph_gc.CompSpecs CompSpecs.
+Defined.
+
+Lemma before_gc_thread_info_rep_fold:
+  forall sh t_info (ti: val),
+  data_at sh env_graph_gc.thread_info_type
+   (offset_val (WORD_SIZE * used_space (heap_head (ti_heap t_info))) (space_start (heap_head (ti_heap t_info))),
+    (offset_val (WORD_SIZE * total_space (heap_head (ti_heap t_info))) (space_start (heap_head (ti_heap t_info))),
+     (ti_heap_p t_info,
+      (ti_args t_info,
+        (spatial_gcgraph.ti_fp t_info, (Vptrofs (ti_nalloc t_info), nullval)))))) ti
+  * spatial_gcgraph.frames_rep sh (ti_frames t_info)
+  * spatial_gcgraph.heap_struct_rep sh
+      ((space_start (heap_head (ti_heap t_info)),
+       (Vundef,
+       (offset_val (WORD_SIZE * total_space (heap_head (ti_heap t_info))) (space_start (heap_head (ti_heap t_info))),
+         offset_val (WORD_SIZE * total_space (heap_head (ti_heap t_info))) (space_start (heap_head (ti_heap t_info))))))
+         :: map spatial_gcgraph.space_tri (tl (spaces (ti_heap t_info))))
+      (ti_heap_p t_info)
+  * spatial_gcgraph.heap_rest_rep (ti_heap t_info) 
+  |-- before_gc_thread_info_rep sh t_info ti.
+Proof.
+ intros.
+ unfold before_gc_thread_info_rep.
+ unfold spatial_gcgraph.before_gc_thread_info_rep.
+ change_compspecs CompSpecs.
+ cancel.
+Qed.
+
+
+Lemma frames_rep_cons:
+ forall vf vr vl frames
+  (SIZE: WORD_SIZE * Zlength vl <= Ptrofs.max_signed),
+ (frame_rep vf vr (spatial_gcgraph.frames_p frames) vl *
+  spatial_gcgraph.frames_rep Tsh frames)%logic
+ = spatial_gcgraph.frames_rep Tsh 
+     ({|fr_adr:=vf; fr_root:=vr; fr_roots := vl|}::frames).
+Proof.
+intros.
+unfold frame_rep.
+simpl.
+unfold tarray.
+unfold spatial_gcgraph.frames_rep.
+unfold frames2rootpairs.
+simpl map.
+change (concat (?A :: ?B)) with (A ++ concat B).
+fold (frames2rootpairs frames).
+unfold spatial_gcgraph.roots_rep.
+rewrite iter_sepcon.iter_sepcon_app_sepcon.
+unfold spatial_gcgraph.frames_shell_rep; fold (spatial_gcgraph.frames_shell_rep Tsh frames).
+unfold frame2rootpairs.
+simpl.
+change gc._stack_frame with _stack_frame.
+match goal with |- ?A = ?B =>
+ transitivity (!! (@field_compatible0 env_graph_gc.CompSpecs (tarray int_or_ptr_type (@Zlength val vl)) [] vr) && A)%logic
+ end.
+ { apply pred_ext; entailer!.
+   apply field_compatible_field_compatible0.
+   unfold tarray.
+   apply field_compatible_change_composite; try apply H1.
+ }
+ normalize.
+ apply andp_prop_ext. tauto.
+ intro.
+ rewrite spatial_gcgraph.iter_sepcon_frame2rootpairs' by auto.
+replace  (field_address0 (tarray int_or_ptr_type (Zlength vl)) (SUB Zlength vl) vr)
+with (offset_val (8 * Zlength vl) vr).
+2:{ unfold field_address0.
+  rewrite if_true. simpl. auto.
+   eapply field_compatible0_cons_Tarray; [ | apply H| ].
+   reflexivity. rep_lia.
+}
+change_compspecs CompSpecs.
+apply pred_ext; cancel.
+Qed.
+
+Lemma frames_rep_push:
+ forall vf vr vl frames
+  (SIZE: WORD_SIZE * Zlength vl <= Ptrofs.max_signed),
+frame_rep vf vr (spatial_gcgraph.frames_p frames) vl *
+spatial_gcgraph.frames_rep Tsh frames
+|-- spatial_gcgraph.frames_rep Tsh 
+     ({|fr_adr:=vf; fr_root:=vr; fr_roots := vl|}::frames).
+Proof.
+intros.
+rewrite frames_rep_cons by auto. auto.
+Qed.
+
+
+Lemma frames_rep_pop:
+ forall vf vr vl frames
+  (SIZE: WORD_SIZE * Zlength vl <= Ptrofs.max_signed),
+ spatial_gcgraph.frames_rep Tsh 
+     ({|fr_adr:=vf; fr_root:=vr; fr_roots := vl|}::frames)
+|-- frame_rep vf vr (spatial_gcgraph.frames_p frames) vl *
+    spatial_gcgraph.frames_rep Tsh frames.
+Proof.
+intros.
+rewrite frames_rep_cons by auto. auto.
+Qed.
+
+Inductive frame_shells_eq: forall frames1 frames2 : list frame, Prop :=
+| fse_nil: frame_shells_eq nil nil
+| fse_cons: forall fr1 fr2 r1 r2,
+    fr_adr fr1 = fr_adr fr2 ->
+    fr_root fr1 = fr_root fr2 ->
+    Zlength (fr_roots fr1) = Zlength (fr_roots fr2) ->
+    frame_shells_eq r1 r2 ->
+    frame_shells_eq (fr1::r1) (fr2::r2).
+
+Definition root_t_of_rep_type (v: rep_type) : root_t :=
+   match v with
+   | repZ i => inl (inl i)
+   | repOut p => inl (inr p)
+   | repNode x => inr x
+  end.
+
+Definition rep_type_of_root_t (v: root_t) : rep_type :=
+  match v with
+  | inl (inl i) => repZ i 
+  | inl (inr p) => repOut p 
+  | inr x => repNode x 
+  end.
+
+Lemma body_uint63_to_nat :
   semax_body Vprog Gprog
              f_uint63_to_nat
              uint63_to_nat_spec.
 Proof. 
 start_function.
-forward. unfold full_gc. Intros. 
+forward. unfold full_gc. Intros.
+ 
 forward_call (gv, g). 
+Intros v.
 assert ( Vlong (Int64.shru (Int64.repr (encode_Z (Z.of_nat n))) (Int64.repr (Int.unsigned (Int.repr 1)))) = Vlong (Int64.repr  (Z.of_nat n)))  as ->.
-  { unfold encode_Z. 
-  autorewrite with norm. Search Int64.shru . rewrite Int64.shru_div_two_p. 
-  unfold two_p.  Search Int64.unsigned Int64.repr. simpl. 
-  
-  admit. (* TODO *)  } 
-(*   Print bool_type. *)
-
-
-
+  { unfold encode_Z in *.
+  f_equal.  
+  autorewrite with norm. rewrite Int64.shru_div_two_p.
+  rewrite !Int64.unsigned_repr by (unfold min_signed, max_signed in *; rep_lia).
+  f_equal.
+  unfold two_p.
+  change (two_power_pos 1) with 2.
+  rewrite Z.div_add_l by lia.
+  simpl. lia.
+ }
+forward.
+forward.
+unfold before_gc_thread_info_rep, spatial_gcgraph.before_gc_thread_info_rep.
+change_compspecs CompSpecs.
+Intros.
+forward.
+   { sep_apply spatial_gcgraph.frames_rep_ptr_or_null. entailer!!. }
+forward.
+sep_apply (frame_rep__fold v___FRAME__ v___ROOT__ (spatial_gcgraph.ti_fp t_info) 1).
+sep_apply before_gc_thread_info_rep_fold.
+sep_apply (full_gc_fold gv g t_info roots outlier ti sh).
 forward_while 
-(EX v : rep_type, EX m : nat, EX g' : graph, EX (t_info' : GCGraph.thread_info),
+(EX v : rep_type, EX m : nat, EX g' : graph, EX (t_info' : GCGraph.thread_info), EX (roots': roots_t),
 PROP (is_in_graph g' m v; (m <= n)%nat;
-gc_graph_iso g roots g' roots)
+gc_condition_prop g' t_info' roots' outlier;
+gc_graph_iso g roots g' roots';
+ti_heap_p t_info'=ti_heap_p t_info; (* not needed? *)
+ti_frames t_info'=ti_frames t_info)
 LOCAL (temp _temp (rep_type_val g' v);
 temp _i (Vlong (Int64.repr (Z.of_nat (n - m))));
-temp _tinfo ti; temp _t (Vlong (Int64.repr (Z.of_nat n))))
-SEP (full_gc g' t_info' roots outlier ti sh)
+   lvar ___FRAME__ (Tstruct _stack_frame noattr) v___FRAME__;
+   lvar ___ROOT__
+     (tarray int_or_ptr_type 1)
+     v___ROOT__; 
+temp _tinfo ti; temp _t (Vlong (Int64.repr (encode_Z (Z.of_nat n))));
+gvars gv)
+SEP (full_gc g' t_info' roots' outlier ti sh gv;
+    frame_rep_ v___FRAME__ v___ROOT__ (spatial_gcgraph.ti_fp t_info') 1;
+    library.mem_mgr gv)
 ). 
 - (* Before the while *)
-  Intros v. Exists v. Exists 0%nat. Exists g. Exists t_info. entailer!. 
-  + split3.
+   Exists v. Exists 0%nat. Exists g. Exists t_info. Exists roots. entailer!. 
+  + split.
     * apply gc_graph_iso_refl.
     * repeat f_equal. lia.
-    * admit. 
-  +  unfold full_gc. entailer!. 
 - (* Valid condition  *)
-  entailer!. 
+  entailer!!. 
 - (* During the loop *)
-  assert (n - m <> 0)%nat.
-  {  destruct (n-m)%nat eqn:EQ_mn; eauto. 
-    simpl in HRE. normalize in HRE. 
-    Print typed_true. unfold typed_true in HRE. simpl in HRE. 
-    unfold Int64.zero in HRE. unfold Int64.eq in HRE. 
-    if_tac in HRE; eauto. simpl in HRE. congruence.
+  rename H4 into GCP. rename H7 into H4.
+  assert (STARTptr: isptr (space_start (heap_head (ti_heap t_info')))). {
+    red in GCP; decompose [and] GCP.
+    destruct (heap_head_cons (ti_heap t_info')) as [s [l [C1 C2]  ] ].
+    rewrite C2.
+    replace s with (Znth 0 (spaces (ti_heap t_info'))) by (rewrite C1; reflexivity).
+    apply space_start_isptr with g'; auto.
+    rewrite C1; clear; list_solve.
+    apply graph_has_gen_O.
   }
-  unfold full_gc. 
+  assert (n - m <> 0)%nat by lia.
+  unfold full_gc.
   unfold before_gc_thread_info_rep.
   unfold spatial_gcgraph.before_gc_thread_info_rep.
-  (* KS: This is where the garbage collector comes in/the proof requires sth different. *)
+  Intros.
+  change_compspecs CompSpecs.
+  forward.
+  forward.
+  destruct (space_start (heap_head (ti_heap t_info'))) eqn:STARTeq; try contradiction.
+  rename b into startb; rename i into starti.
+  forward_if (
+     EX g'': graph, EX v0':_, EX roots':_, EX t_info' : GCGraph.thread_info,
+     PROP ( total_space (heap_head (ti_heap t_info')) - used_space (heap_head (ti_heap t_info')) >= 2;
+            is_in_graph g'' m v0';
+            gc_condition_prop g'' t_info' roots' outlier;
+            gc_graph_iso g roots g'' roots';
+            ti_heap_p t_info'=ti_heap_p t_info; (* not needed?*)
+            ti_frames t_info'=ti_frames t_info) (* not needed? *)
+     LOCAL (temp _temp (rep_type_val g'' v0');
+     temp _i (Vlong (Int64.repr (Z.of_nat (n-m))));
+     lvar ___FRAME__ (Tstruct _stack_frame noattr) v___FRAME__;
+     lvar ___ROOT__ (tarray int_or_ptr_type 1) v___ROOT__; 
+     temp _tinfo ti; temp _t (Vlong (Int64.repr (encode_Z (Z.of_nat n))));
+     gvars gv)
+     SEP (full_gc g'' t_info' roots' outlier ti sh gv;
+          frame_rep_ v___FRAME__ v___ROOT__ (spatial_gcgraph.ti_fp t_info') 1;
+          library.mem_mgr gv))%assert.
+ + apply prop_right; simpl. destruct (peq startb startb); try contradiction. auto.
+ +
+  forward.
+  forward.
+  unfold frame_rep_. Intros.
+  forward.
+  forward.
+  deadvars!.
+  change (upd_Znth 0 _ _) with ([rep_type_val g' v0]).
+  change (Tpointer tvoid _) with int_or_ptr_type.
+  assert_PROP (force_val (sem_add_ptr_int int_or_ptr_type Signed v___ROOT__ (Vint (Int.repr 1))) =
+      offset_val (sizeof int_or_ptr_type * 1) v___ROOT__)  as H99; [ entailer! | rewrite H99; clear H99].
+  sep_apply (frame_rep_fold v___FRAME__ v___ROOT__ (spatial_gcgraph.ti_fp t_info') 1 [rep_type_val g' v0]).
+  unfold spatial_gcgraph.ti_fp.
+  replace (spatial_gcgraph.frames_rep sh) with (spatial_gcgraph.frames_rep Tsh)
+     by admit.  (* This needs fixing *)
+  sep_apply (frames_rep_cons v___FRAME__ v___ROOT__ [rep_type_val g' v0] (ti_frames t_info')).
+  compute; clear; congruence.
+  set (frames'' := _ :: ti_frames t_info').
+  pose (t_info'' := {| ti_heap_p := ti_heap_p t_info'; ti_heap := ti_heap t_info';
+                      arg_size := arg_size t_info'; ti_frames := frames'';
+                      ti_nalloc := Ptrofs.repr 2 |}).
+  change frames'' with (ti_frames t_info'').
+  rewrite Int.signed_repr by rep_lia.
+  change (ti_args t_info') with (ti_args t_info'').
+  change (ti_heap_p t_info') with (ti_heap_p t_info'').
+  clear H8.
+  forward_call (Ers, sh, gv, ti, g', t_info'', root_t_of_rep_type v0 :: roots', outlier).
+  *
+   unfold spatial_gcgraph.before_gc_thread_info_rep.
+   change_compspecs CompSpecs.
+   replace (spatial_gcgraph.frames_rep sh) with (spatial_gcgraph.frames_rep Tsh)
+      by admit.  (* This needs fixing *)
+   rewrite <- STARTeq.
+   change (ti_heap t_info') with (ti_heap t_info'').
+   cancel.
+  * simpl.
+    split3.
+    red. red in GCP.
+    split3; [ tauto | | split; [ | tauto] ].
+    --
+     subst frames''; clear t_info''.
+     unfold frames2rootpairs. simpl concat.
+     unfold rootpairs_compatible. simpl.
+     f_equal.  destruct v0; auto.
+     change (rootpairs_compatible g' (frames2rootpairs (ti_frames t_info')) roots').
+     tauto.
+    -- decompose [and] GCP; clear GCP. destruct H15.
+       split. 
+       ++ clear t_info'' frames'' H7 STARTptr STARTeq startb starti H3 HRE' HRE.
+          admit.  (* problematic . . . 
+          intros ? ? . destruct v0; auto.  destruct H3; auto. subst a.
+          red in H2. hnf in H2.   
+           *)
+       ++ destruct v0; try apply H18. constructor; auto.
+          clear - H2. unfold is_in_graph in H2.
+          apply has_v in H2; auto.
+    -- red in GCP; decompose [and] GCP; split; auto.
+    -- apply GCP.
+  * (* after the call to garbage_collect() *)
+   Intros vret. destruct vret as [ [g3 t_info3] roots3].
+   simpl snd in *. simpl fst in *.
+   forward.
+   unfold spatial_gcgraph.before_gc_thread_info_rep.
+   replace (spatial_gcgraph.frames_rep sh) with (spatial_gcgraph.frames_rep Tsh)
+   by admit.  (* This needs fixing *)
 
-
-  (* Old proof: 
-  forward_call (gv, g', [v], (m%nat; tt) , roots, sh, ti, outlier, t_info'). 
-  { (* Requiring to unfold. *)
-    admit. }
-  Intros v'.  destruct v' as ((v'&g'')&ti').
-  unfold fst, snd in *. 
-  forward. 
-  Exists (v', S m, g'', ti').
-  (* Don't know why this is diverging - this used to work. *)
-  
-  (*  entailer!. 
-  split; eauto. 
-  + eapply gc_graph_iso_trans; eauto.  
-  + repeat f_equal.  lia.  *) 
-  admit. *)
-
--
-(* TODO:     Diverges for some reason. 
-  forward. 
-  { unfold full_gc. entailer!.  }
-
-  Exists v. Exists g'. Exists t_info0.
-  entailer!. 
-
-  enough (n- m = 0)%nat. 
-  { assert (n = m) by lia. subst. eauto. }
-  red in HRE.  
-  unfold strict_bool_val in HRE. simpl in HRE. 
-unfold Int64.zero in HRE. 
-  Search (Int64.eq (Int64.repr _) (Int64.repr _)).
-  clear -HRE.
-
-  destruct (n-m)%nat eqn:EQ_mn; eauto. 
-  simpl in HRE. normalize in HRE. 
-  unfold typed_false in HRE. simpl in HRE. 
-  unfold Int64.eq in HRE. if_tac in HRE; simpl in *; try congruence. 
-  revert H6. Search Int64.unsigned Int64.zero. 
-  rewrite Int64.unsigned_zero.
-  admit. *)
-admit. 
-Admitted.
+   assert (FSE: frame_shells_eq (ti_frames t_info'') (ti_frames t_info3)) 
+       by admit. (* should be a postcondition of garbage_collect *)
+    simpl in FSE. unfold frames'' in FSE.
+    remember (ti_frames t_info3) as frames3.
+    inversion FSE; clear FSE. subst r1 fr1.
+    destruct fr2 as [a3 r3 s3]; simpl in H14, H15, H16.
+    subst a3 r3.
+    destruct s3. exfalso; clear - H16; list_solve.
+    destruct s3. 2: exfalso; clear - H16; list_solve.
+    subst frames3.
+    sep_apply (frames_rep_pop v___FRAME__ v___ROOT__ [v1] r2).
+    compute; clear; congruence.
+    unfold frame_rep at 1.
+    Intros. change (Zlength [_]) with 1.
+    assert (roots_graph_compatible (root_t_of_rep_type v0 :: roots') g') by admit.
+    assert (ISO: gc_graph_iso g' (root_t_of_rep_type v0 :: roots') g3 roots3). {
+     red in H8; decompose [and] H8.
+     apply garbage_collect_isomorphism; auto; try apply GCP.
+    }
+    assert (exists v0', exists roots3',
+        v1 = rep_type_val g3 v0' /\ is_in_graph g3 m v0' /\ roots3 = root_t_of_rep_type v0' :: roots3'). {
+     destruct ISO as [f12 [f21 [e12 [e21 [? ?] ] ] ] ].
+     simpl in H13.
+     subst roots3.
+     exists (rep_type_of_root_t (root_map f12 (root_t_of_rep_type v0))).
+     eexists.
+     split3. 3: simpl; f_equal; try reflexivity.
+     3: subst 
+     + admit.  (* Maybe;  graph_isomorphism property *)     
+     + admit.  (* Maybe *)
+     + admit. (* easy *)
+     + destruct v0; auto.
+    }
+    destruct H13 as [v0' [roots3' [ ? [? ?] ] ] ].
+    subst v1 roots3.
+    forward. entailer!!. rewrite Znth_0_cons. 
+        admit. (* easy *)
+    forward.  entailer!!. 
+        admit. (* easy *)
+    change_compspecs CompSpecs.
+    forward.
+    pose (t_info4 := {|
+      ti_heap_p := ti_heap_p t_info3;
+      ti_heap := ti_heap t_info3;
+      ti_args := ti_args t_info3;
+      arg_size := arg_size t_info3;
+      ti_frames := r2;
+      ti_nalloc := ti_nalloc t_info3
+    |} ).
+    Exists g3 v0' roots3' t_info4.
+    rewrite Znth_0_cons.
+    unfold full_gc.
+    entailer!!.
+    -- admit.
+    -- unfold before_gc_thread_info_rep, spatial_gcgraph.before_gc_thread_info_rep, frame_rep_.
+      change_compspecs CompSpecs.
+      replace (spatial_gcgraph.frames_rep sh) with (spatial_gcgraph.frames_rep Tsh)
+      by admit.  (* This needs fixing *)
+      unfold spatial_gcgraph.ti_fp. 
+      unfold t_info4; simpl.
+      replace (Vlong (Ptrofs.to_int64 (ti_nalloc t_info3))) with (Vptrofs (ti_nalloc t_info3))
+        by (rewrite Vptrofs_unfold_true by reflexivity; reflexivity).
+      cancel.
+      unfold frame_rep_surplus. change (1 - Zlength _) with 0.
+      Intros.
+      sep_apply data_at__data_at.
+      sep_apply data_at_zero_array_eq. 
+           admit. (* easy *)
+      do 2 unfold_data_at (data_at _ (Tstruct _stack_frame noattr) _ _).
+      cancel.
+  + forward.
+    Exists g' v0 roots t_info'.
+    unfold full_gc, before_gc_thread_info_rep, spatial_gcgraph.before_gc_thread_info_rep.
+    rewrite <- STARTeq.
+    change_compspecs CompSpecs.
+    entailer!!.
+    admit.  (* from typed_false tint ... *)
+  + Intros g4 v0' roots4 t_info4.
+  pose (m' := existT (fun _ => unit) m tt).
+  forward_call (gv, g4, [v0'], m', roots4, sh, ti, outlier, t_info4).
+   * split.
+      split; auto. reflexivity. 
+      admit.  (* OK *)
+   * Intros vret.
+     destruct vret as [ [ v2 g5] t_info5].
+     simpl snd in *. simpl fst in *.
+     assert (MISSING: ti_heap_p t_info5 = ti_heap_p t_info /\ 
+             ti_frames t_info5 = ti_frames t_info4 /\
+             gc_condition_prop g5 t_info5 roots4 outlier) by admit. (* missing from postcondition? *)
+     destruct MISSING as [ M1 [M2 GCP'] ].
+     simpl in H13.
+     forward.
+     Exists (v2, S m,g5,t_info5,roots4). simpl fst. simpl snd.
+     unfold spatial_gcgraph.ti_fp.
+     replace (Z.of_nat (n - S m)) with (Z.of_nat (n-m)-1) by lia.
+     rewrite M1, M2.
+     entailer!!.
+     eapply gc_graph_iso_trans; eassumption.
+ - (* after the loop *)
+   forward.
+   assert (m=n). {
+    clear - H3 H HRE. unfold encode_Z in H. unfold min_signed, max_signed in H. simpl in H.
+    apply repr_inj_unsigned64 in HRE; try rep_lia.     
+   }
+   subst m.
+   Exists v0 g' t_info' roots'.
+   unfold frame_rep_.
+   entailer!!.
+all:fail.
+Admitted. 
